Some proof progress

ironfleet/src/Dafny/Distributed/Protocol/FailureDetector/Proof.i.dfy
@@ -1,12 +1,173 @@
-include "DistributedSystem.dfy"
+include "TimestampedDistributedSystem.i.dfy"
 
+module FailureDetector_Proof {
+import opened FailureDetector_TimestampedDistributedSystem
 
-module FailureDetector_Detector {
-import opened FailureDetector_DistributedSystem
+ghost const FailureTime:Timestamp
+ghost const TimeoutInterval:Timestamp
 
+predicate BoundedQueueingAssumption(s:TFD_State)
+{
+    && s.t_environment.nextStep.LEnvStepHostIos?
+    ==>
+  var ios := s.t_environment.nextStep.ios;
+    (forall io :: io in s.t_environment.nextStep.ios && io.LIoOpReceive? && io.r.dst in s.t_servers ==>
+
+      // this means that max(replica.ts, msg.ts) <= msg.ts + MaxQueueTime
+      s.t_servers[io.r.dst].ts <= io.r.msg.ts + Q
+    )
+}
+
+//
 predicate Assumption(s:TFD_State)
 {
+  BoundedQueueingAssumption(s)
 
+  && (forall i :: i in s.t_servers ==>
+    TimeLe(s.t_servers[i].ts, FailureTime)
+    && (s.t_servers[i].v.N? ==> s.t_servers[i].v.n.state == RUNNING)
+    && (s.t_servers[i].v.D? ==> s.t_servers[i].v.d.timeoutInterval == TimeoutInterval)
+    // FIXME: assume that RUNNING ==> ts <= FailureTime()
+   )
+}
+
+predicate ClockAssumption(s:TFD_State)
+{
+  true
+}
+
+// inductive on its own
+predicate BasicInvariant(s:TFD_State)
+{
+  && |s.t_servers| == 2
+    && s.config.nodeEp in s.t_servers
+    && s.config.detectorEp in s.t_servers
+    && s.t_servers[s.config.detectorEp].v.D?
+    && s.t_servers[s.config.nodeEp].v.N?
+    && s.t_servers[s.config.detectorEp].v.D?
+}
+
+function LastHBDeliveryTime() : Timestamp
+{
+  FailureTime + MbeSend + Delay
+}
+
+function FailureDetectionTime() : Timestamp
+{
+  FailureTime + MbeSend + Delay + Q + TimeoutInterval
+}
+
+predicate Guarantee(s:TFD_State)
+{
+  && (forall pkt :: pkt in s.t_environment.sentPackets && pkt.msg.v.Alert? ==>
+    TimeLe(pkt.msg.ts, LastHBDeliveryTime())
+    )
+}
+
+datatype FailState =
+  | NotFailed
+  | Failed(pkt:TimestampedLPacket<EndPoint,FDMessage>)
+
+predicate Invariant_aux(s:TFD_State, fs:FailState)
+  requires BasicInvariant(s)
+{
+  && (forall pkt :: pkt in s.t_environment.sentPackets && pkt.msg.v.Heartbeat? ==>
+    TimeLe(pkt.msg.ts, LastHBDeliveryTime())
+    )
+    && (
+    if fs.Failed? then
+    (fs.pkt in s.t_environment.sentPackets && fs.pkt.msg.v.Alert?
+       && TimeLe(fs.pkt.msg.ts, FailureDetectionTime()))
+    else
+      (forall pkt :: pkt in s.t_environment.sentPackets ==> pkt.msg.v.Alert? ==> false)
+      && s.t_servers[s.config.detectorEp].v.d.lastHeartbeatTime <= (LastHBDeliveryTime() + Q)
+    )
+}
+
+lemma InvInductiveDetector_0(s:TFD_State, s':TFD_State, fs:FailState)
+  requires Assumption(s)
+  requires Assumption(s')
+  requires s.t_environment.nextStep.LEnvStepHostIos?;
+  requires s.t_environment.nextStep.actor == s.config.detectorEp;
+  requires s.t_environment.nextStep.nodeStep == DetectorStep(0)
+  requires TFD_NextOneServer(s, s', s.t_environment.nextStep.actor, s.t_environment.nextStep.ios);
+  requires BasicInvariant(s)
+  requires BasicInvariant(s')
+
+  requires Invariant_aux(s, fs)
+  ensures Invariant_aux(s', fs)
+{
+  var ios := s.t_environment.nextStep.ios;
+  if ios[0].LIoOpReceive? && ios[0].r.msg.v.Heartbeat? {
+    assert ios[1].t <= s'.t_servers[s.config.detectorEp].ts;
+    assert ios[1].t <= (LastHBDeliveryTime() + Q);
+  } else {
+
+  }
+}
+
+lemma InvInductiveDetector_1(s:TFD_State, s':TFD_State, fs:FailState) returns (fs':FailState)
+  requires Assumption(s)
+  requires Assumption(s')
+  requires s.t_environment.nextStep.LEnvStepHostIos?;
+  requires s.t_environment.nextStep.actor == s.config.detectorEp;
+  requires s.t_environment.nextStep.nodeStep == DetectorStep(1)
+  requires TFD_NextOneServer(s, s', s.t_environment.nextStep.actor, s.t_environment.nextStep.ios);
+  requires BasicInvariant(s)
+  requires BasicInvariant(s')
+
+  requires Invariant_aux(s, fs)
+  ensures Invariant_aux(s', fs')
+{
+  var ios := s.t_environment.nextStep.ios;
+  if fs.Failed? {
+    fs' := fs;
+  } else {
+    var sentPackets := ExtractSentPacketsFromIos(UntagLIoOpSeq(ios));
+    if |sentPackets| > 0 {
+      var ios_u := UntagLIoOpSeq(ios);
+      assert SpontaneousIos(ios_u, 1);
+      assert sentPackets[0] in sentPackets; // XXX: Here to trigger ensures of ExtractSentPacketsFromIos
+      assert 1 < |ios_u|;
+      assert ios_u[1].LIoOpSend?;
+      assert ios[1].LIoOpSend?;
+      fs' := Failed(ios[1].s);
+    } else {
+      fs' := NotFailed;
+      assert (forall pkt :: pkt in s'.t_environment.sentPackets ==> pkt.msg.v.Alert? ==> false);
+      assert s.t_servers[s'.config.detectorEp].v.d.lastHeartbeatTime == s'.t_servers[s'.config.detectorEp].v.d.lastHeartbeatTime;
+      //assert s'.t_servers[s'.config.detectorEp].v.d.lastHeartbeatTime <= LastHBDeliveryTime();
+    }
+  }
+}
+
+
+lemma {:verify false} InvInductive(s:TFD_State, s':TFD_State, actor:EndPoint, fs:FailState) returns (fs':FailState)
+  requires Assumption(s)
+  requires Assumption(s')
+  requires s.t_environment.nextStep.LEnvStepHostIos?;
+  requires s.t_environment.nextStep.actor == actor
+  requires TFD_NextOneServer(s, s', s.t_environment.nextStep.actor, s.t_environment.nextStep.ios);
+  requires BasicInvariant(s)
+  requires BasicInvariant(s')
+
+  requires Invariant_aux(s, fs)
+  ensures Invariant_aux(s', fs')
+{
+  if fs.Failed? {
+    fs' := fs;
+    if actor == s.config.nodeEp {
+      assert
+        && (forall pkt :: pkt in s'.t_environment.sentPackets && pkt.msg.v.Heartbeat? ==>
+        TimeLe(pkt.msg.ts, LastHBDeliveryTime())
+        );
+      assume false;
+    } else {
+      assume actor == s.config.detectorEp;
+    }
+  } else {
+    assume false;
+  }
 }
 
 }
