ironfleet/src/Dafny/Distributed/Protocol/FailureDetector/TimestampedDistributedSystem.i.dfy
@@ -5,6 +5,30 @@ module FailureDetector_TimestampedDistributedSystem {
 import opened FDTimestampedEnv_s
 import opened FailureDetector_DistributedSystem
 
+ghost const Delay:Timestamp
+ghost const Q:Timestamp
+
+ghost const TryRecv:Timestamp
+ghost const MbeTimeout:Timestamp
+ghost const MbeSend:Timestamp
+ghost const Unknown:Timestamp
+
+predicate TimeLe(lhs:Timestamp, rhs:Timestamp)
+{
+  lhs <= rhs
+}
+
+function StepToTimeDelta(hstep:FDStep) : Timestamp
+{
+  if hstep == NodeStep then
+    MbeSend
+  else if hstep == DetectorStep(0) then
+    TryRecv
+  else if hstep == DetectorStep(1) then
+    MbeTimeout
+  else
+    Unknown
+}
 
 type TimestampedAgent = TimestampedType<Agent>
 
@@ -30,10 +54,44 @@ datatype TFD_State = TFD_State(
       && forall id :: id in s.t_servers ==> s.t_servers[id].ts == TimeZero()
   }
 
-  predicate TFD_NextOneServer(s:TFD_State, s':TFD_State, actor:EndPoint, ios:seq<TimestampedLIoOp<EndPoint, FDMessage>>, hstep:FDStep)
+  function FD_NoRecvPerfUpdate(node_pr:Timestamp, hstep:FDStep) : Timestamp
   {
+    var total_time := TimeAdd2(node_pr, StepToTimeDelta(hstep));
+    total_time
+  }
+
+  function FD_RecvPerfUpdate(node_ts:Timestamp, pkt_ts:Timestamp, hstep:FDStep) : Timestamp
+  {
+    var handlerStartTime := TimeMax(pkt_ts, node_ts);
+    var total_time := TimeAdd2(handlerStartTime, StepToTimeDelta(hstep));
+    total_time
+  }
+
+  function FD_TimeoutPerfUpdate(node_ts:Timestamp, hstep:FDStep) : Timestamp
+  {
+    node_ts + Timeout() + StepToTimeDelta(hstep)
+  }
+
+  predicate TFD_NextOneServer(s:TFD_State, s':TFD_State, actor:EndPoint, ios:seq<TimestampedLIoOp<EndPoint, FDMessage>>)
+  {
+    && s.config == s'.config
     && actor in s.t_servers
     && FD_NextOneServer(UntagFDState(s), UntagFDState(s'), actor, UntagLIoOpSeq(ios))
-      && s.t_environment.nextStep.nodeStep == hstep
+    && LEnvironment_Next(s.t_environment, s'.t_environment)
+
+    && var hstep := s.t_environment.nextStep.nodeStep;
+    (if |ios| > 0 && ios[0].LIoOpReceive? then
+      && ios[0] in ios
+      && TimeLe(s'.t_servers[actor].ts, FD_RecvPerfUpdate(s.t_servers[actor].ts, ios[0].r.msg.ts, hstep))
+      && (ios[0].r.msg.ts <= s.t_servers[actor].ts + Timeout())
+    else if |ios| > 0 && ios[0].LIoOpTimeoutReceive? then
+      && TimeLe(s'.t_servers[actor].ts, FD_TimeoutPerfUpdate(s.t_servers[actor].ts, hstep))
+    else
+      && TimeLe(s'.t_servers[actor].ts, FD_NoRecvPerfUpdate(s.t_servers[actor].ts, hstep))
+      )
+
+      && (forall io :: io in ios && io.LIoOpSend? ==>
+          TimeLe(io.s.msg.ts, s'.t_servers[actor].ts + Delay)
+      )
   }
 }
